src/typechecker/FStar.TypeChecker.Core.fsti
@@ -10,8 +10,12 @@ val clear_memo_table (_:unit)
   : unit
 
 val error : Type0
-
+  
 val check_term (g:Env.env) (e:term) (t:typ) (must_tot:bool)
+  : either (option typ) error
+
+(* for unit testing *)
+val check_term_equality (g:Env.env) (t0 t1:typ)
   : either (option typ) error
 
 val print_error (err:error)
